store/impl.v
@@ -5,8 +5,7 @@ From iris.algebra Require Import agree auth csum gset gmap excl frac.
 From iris.algebra Require Import max_prefix_list.
 From iris.heap_lang Require Import notation proofmode.
 From iris.heap_lang.lib Require Import lock ticket_lock.
-From cryptis Require Import lib version term cryptis primitives tactics.
-From cryptis Require Import role iso_dh.
+From cryptis Require Import lib version term cryptis primitives tactics conn.
 From cryptis.store Require Import alist db.
 
 Set Implicit Arguments.
@@ -15,170 +14,6 @@ Unset Printing Implicit Defensive.
 
 Local Existing Instance ticket_lock.
 
-(* MOVE *)
-Definition list_hd : val := λ: "l",
-  match: "l" with
-    NONE => NONE
-  | SOME "l" => Fst "l"
-  end.
-
-Definition list_tl : val := λ: "l",
-  match: "l" with
-    NONE => NONE
-  | SOME "l" => Snd "l"
-  end.
-
-Lemma repr_listE `{Repr A} (l : list A) :
-  repr l =
-  match l with
-  | [] => NONEV
-  | x :: xs => SOMEV (repr x, repr xs)
-  end.
-Proof.
-rewrite /= repr_list_unseal. by case: l.
-Qed.
-(* /MOVE *)
-
-Module Connection.
-
-Section Connection.
-
-Variable N : namespace.
-
-Definition session_key : val := λ: "cs",
-  Snd "cs".
-Definition connect : val := λ: "c" "skA" "vkB",
-  let: "session_key" :=
-    do_until (λ: <>, initiator (N.@"auth") "c" "skA" "vkB") in
-  let: "timestamp" := ref #0%nat in
-  let: "m" := senc (N.@"init") "session_key" (TInt 0) in
-  send "c" "m";;
-  do_until (λ: <>,
-    let: "m" := recv "c" in
-    sdec (N.@"ack_init") "session_key" "m");;
-  ("timestamp", "session_key").
-
-Definition listen : val := λ: "c" "skA",
-  let: "result" := do_until (λ: <>, responder (N.@"auth") "c" "skA") in
-  let: "timestamp" := ref #0 in
-  let: "vkB" := Fst "result" in
-  let: "session_key" := Snd "result" in
-  do_until (λ: <>,
-    let: "m" := recv "c" in
-    sdec (N.@"init") "session_key" "m");;
-  ("vkB", ("timestamp", "session_key")).
-
-Definition confirm : val := λ: "c" "cs",
-  let: "sk" := Snd "cs" in
-  let: "m"  := senc (N.@"ack_init") "sk" (TInt 0) in
-  send "c" "m".
-
-Definition timestamp : val := λ: "cs",
-  let: "timestamp" := Fst "cs" in
-  !"timestamp".
-
-Definition tick : val := λ: "cs",
-  let: "timestamp" := Fst "cs" in
-  "timestamp" <- (!"timestamp" + #1).
-
-Definition write N : val := λ: "c" "cs" "ts",
-  let: "n"  := timestamp "cs" in
-  let: "sk" := session_key "cs" in
-  let: "m"  := term_of_list (tint "n" :: "ts") in
-  let: "m"  := senc N "sk" "m" in
-  send "c" "m".
-
-Definition make_handler (p : namespace * expr) : expr :=
-  let N := p.1 in
-  let: "handler" := p.2 in
-  λ: "n" "m",
-    bind: "m" := untag N "m" in
-    bind: "ts" := list_of_term "m" in
-    match: "ts" with
-      NONE => NONE
-    | SOME "ts" =>
-      bind: "n'" := to_int (Fst "ts") in
-      guard: "n" = "n'" in
-      "handler" (Snd "ts")
-    end.
-
-Lemma subst_make_handler var v p :
-  subst var v (make_handler p) =
-  make_handler (p.1, subst var v p.2).
-Proof.
-case: p => [N' handler] /=.
-case: decide => [[_ not_shadow_handler]|shadow_handler //].
-case: decide => [[_ not_shadow_n]|shadow_n //].
-case: decide => [[_ not_shadow_m]|shadow_m //].
-rewrite decide_False; last congruence.
-case: decide => [[_ not_shadow_ts]|shadow_ts //].
-rewrite decide_False; last congruence.
-case: decide => [[_ not_shadow_n']|shadow_n' //].
-rewrite decide_False; last congruence.
-rewrite decide_False; last congruence.
-by rewrite decide_False; last congruence.
-Qed.
-
-Fixpoint make_handlers (handlers : list (namespace * expr)) : expr :=
-  match handlers with
-  | [] => []%E
-  | handler :: handlers => (make_handler handler :: make_handlers handlers)%E
-  end.
-
-Lemma subst_make_handlers var v handlers :
-  subst var v (make_handlers handlers) =
-  make_handlers (map (λ p, (p.1, subst var v p.2)) handlers).
-Proof.
-elim: handlers=> [|p handlers IH] //=.
-by rewrite -IH -subst_make_handler.
-Qed.
-
-Definition select_body : val := rec: "loop" "ts" "m" "handlers" :=
-  match: "handlers" with
-    NONE => NONE
-  | SOME "handlers" =>
-    let: "handler" := Fst "handlers" in
-    let: "handlers" := Snd "handlers" in
-    match: "handler" "ts" "m" with
-      NONE => "loop" "ts" "m" "handlers"
-    | SOME "res" => SOME "res"
-    end
-  end.
-
-Definition select_def (c cs : expr) handlers : expr :=
-  (λ: "c" "cs" "handlers",
-    let: "ts" := timestamp "cs" in
-    let: "sk" := session_key "cs" in
-    do_until (λ: <>,
-      let: "m" := recv "c" in
-      bind: "m" := open (key Open "sk") "m" in
-      select_body "ts" "m" "handlers"
-    ))%V c cs (make_handlers handlers).
-
-Definition select_aux : base.seal select_def. by eexists _. Qed.
-Definition select := unseal select_aux.
-Lemma select_eq : select = select_def. Proof. exact: seal_eq. Qed.
-
-Definition read N : val :=
-  let handlers := [(N, (λ: "ts", SOME "ts")%E)] in
-  λ: "c" "cs", select "c" "cs" handlers.
-
-Lemma subst_select var v c cs handlers :
-  subst var v (select c cs handlers) =
-  select (subst var v c) (subst var v cs)
-         (map (λ p, (p.1, subst var v p.2)) handlers).
-Proof.
-by rewrite select_eq /select /= subst_make_handlers.
-Qed.
-
-Definition close : val := λ: "c" "cs",
-  let: "timestamp" := Fst "cs" in
-  Free "timestamp".
-
-End Connection.
-
-End Connection.
-
 Module Client.
 
 Section Client.
@@ -186,31 +21,31 @@ Section Client.
 Variable N : namespace.
 
 Definition connect : val := λ: "c" "skA" "vkB",
-  Connection.connect N "c" "skA" "vkB".
+  Conn.connect N "c" "skA" "vkB".
 
 Definition store : val := λ: "c" "cs" "k" "v",
-  Connection.write (N.@"store") "c" "cs" ["k"; "v"];;
-  Connection.read (N.@"ack_store") "c" "cs";;
-  Connection.tick "cs".
+  Conn.write (N.@"store") "c" "cs" ["k"; "v"];;
+  Conn.read (N.@"ack_store") "c" "cs";;
+  Conn.tick "cs".
 
 Definition load : val := λ: "c" "cs" "k",
-  Connection.write (N.@"load") "c" "cs" ["k"];;
-  let: "ts" := Connection.read (N.@"ack_load") "c" "cs" in
-  Connection.tick "cs";;
+  Conn.write (N.@"load") "c" "cs" ["k"];;
+  let: "ts" := Conn.read (N.@"ack_load") "c" "cs" in
+  Conn.tick "cs";;
   match: "ts" with
     NONE => TInt 0
   | SOME "ts" => Fst "ts"
   end.
 
 Definition create : val := λ: "c" "cs" "k" "v",
-  Connection.write (N.@"create") "c" "cs" ["k"; "v"];;
-  Connection.read (N.@"ack_create") "c" "cs";;
-  Connection.tick "cs".
+  Conn.write (N.@"create") "c" "cs" ["k"; "v"];;
+  Conn.read (N.@"ack_create") "c" "cs";;
+  Conn.tick "cs".
 
 Definition close : val := λ: "c" "cs",
-  Connection.write (N.@"close") "c" "cs" [];;
-  Connection.read (N.@"ack_close") "c" "cs";;
-  Connection.close "c" "cs".
+  Conn.write (N.@"conn".@"close") "c" "cs" [];;
+  Conn.read (N.@"conn".@"ack_close") "c" "cs";;
+  Conn.close "c" "cs".
 
 End Client.
 
@@ -228,8 +63,8 @@ Definition handle_store N : val :=
 λ: "c" "cs" "db" "req",
   list_match: ["k"; "v"] := "req" in
   SAList.insert "db" "k" "v";;
-  Connection.write (N.@"ack_store") "c" "cs" [];;
-  Connection.tick "cs";;
+  Conn.write (N.@"ack_store") "c" "cs" [];;
+  Conn.tick "cs";;
   SOME #true.
 
 (* FIXME: Should return an error when the key is not present *)
@@ -237,8 +72,8 @@ Definition handle_load N : val :=
 λ: "c" "cs" "db" "req",
   list_match: ["k"] := "req" in
   bind: "data" := SAList.find "db" "k" in
-  Connection.write (N.@"ack_load") "c" "cs" ["data"];;
-  Connection.tick "cs";;
+  Conn.write (N.@"ack_load") "c" "cs" ["data"];;
+  Conn.tick "cs";;
   SOME #true.
 
 Definition handle_create N : val :=
@@ -252,14 +87,14 @@ Definition handle_create N : val :=
       #1
     end in
   let: "m" := ["k"; "v"; tint "success"] in
-  Connection.write (N.@"ack_create") "c" "cs" "m";;
-  Connection.tick "cs";;
+  Conn.write (N.@"ack_create") "c" "cs" "m";;
+  Conn.tick "cs";;
   SOME #true.
 
 Definition handle_close N : val :=
 λ: "c" "cs" "db" "req",
-  Connection.write (N.@"ack_close") "c" "cs" [TInt 0];;
-  Connection.close "c" "cs";;
+  Conn.write (N.@"conn".@"ack_close") "c" "cs" [TInt 0];;
+  Conn.close "c" "cs";;
   SOME #false.
 
 Definition conn_handler_body N : val :=
@@ -267,9 +102,9 @@ Definition conn_handler_body N : val :=
     (N.@"store", handle_store N "c" "cs" "db");
     (N.@"load", handle_load N "c" "cs" "db");
     (N.@"create", handle_create N "c" "cs" "db");
-    (N.@"close", handle_close N "c" "cs" "db")
+    (N.@"conn".@"close", handle_close N "c" "cs" "db")
   ] in λ: "c" "cs" "db",
-     Connection.select "c" "cs" handlers.
+     Conn.select "c" "cs" handlers.
 
 Definition conn_handler N : val := rec: "loop" "c" "cs" "db" "lock" :=
   if: conn_handler_body N "c" "cs" "db" then
@@ -290,14 +125,14 @@ Definition find_client : val := λ: "ss" "client_key",
 Definition listen N : val := λ: "c" "ss",
   let: "secret_key" := Fst "ss" in
   let: "clients" := Snd "ss" in
-  let: "res" := Connection.listen N "c" "secret_key" in
+  let: "res" := Conn.listen N "c" "secret_key" in
   let: "client_key" := Fst "res" in
   let: "cs" := Snd "res" in
   let: "account" := find_client "ss" "client_key" in
   let: "db" := Fst "account" in
   let: "lock" := Snd "account" in
   acquire "lock";;
-  Connection.confirm N "c" "cs";;
+  Conn.confirm N "c" "cs";;
   Fork (conn_handler N "c" "cs" "db" "lock").
 
 End Server.
