store/shared.v
@@ -8,8 +8,7 @@ From iris.base_logic.lib Require Import invariants.
 From iris.heap_lang Require Import notation proofmode.
 From iris.heap_lang.lib Require Import ticket_lock.
 From cryptis Require Import lib version term gmeta nown.
-From cryptis Require Import cryptis primitives tactics.
-From cryptis Require Import role iso_dh.
+From cryptis Require Import cryptis primitives tactics role iso_dh conn.
 From cryptis.store Require Import alist db.
 
 Set Implicit Arguments.
@@ -17,18 +16,6 @@ Unset Strict Implicit.
 Unset Printing Implicit Defensive.
 
 Local Existing Instance ticket_lock.
-
-Record conn_state := ConnState {
-  cs_si   :> sess_info;
-  cs_ts   :  loc;
-  cs_role :  role;
-}.
-
-Definition cs_share cs := si_share_of (cs_role cs) cs.
-
-#[global]
-Instance cs_repr : Repr conn_state :=
-  λ s, (#(cs_ts s), si_key s)%V.
 
 Record server_state := {
   ss_key : term;
@@ -49,19 +36,17 @@ Record server_client_state := {
 Instance scs_repr : Repr server_client_state :=
   λ s, (scs_db s, scs_lock s)%V.
 
-Definition statusR := dfrac_agreeR natO.
-
 Class storeGS Σ := StoreGS {
-  storeGS_db      : dbGS Σ;
-  storeGS_status  : inG Σ statusR;
+  storeGS_db   : dbGS Σ;
+  storeGS_conn : Conn.connGS Σ;
 }.
 
 Local Existing Instance storeGS_db.
-Local Existing Instance storeGS_status.
+Local Existing Instance storeGS_conn.
 
 Definition storeΣ := #[
   dbΣ;
-  GFunctor statusR
+  Conn.connΣ
 ].
 
 Global Instance subG_storeGS Σ : subG storeΣ Σ → storeGS Σ.
@@ -72,325 +57,41 @@ Section Defs.
 Context `{!cryptisGS Σ, !heapGS Σ, !storeGS Σ, !tlockG Σ}.
 Notation iProp := (iProp Σ).
 
-Implicit Types (cs : conn_state).
+Implicit Types (si : sess_info).
+Implicit Types (cs : Conn.state).
 Implicit Types (kI kR kS t : term) (ts : list term).
 Implicit Types db : gmap term term.
 Implicit Types accounts : gmap term server_client_state.
 Implicit Types n : nat.
 Implicit Types b : bool.
-Implicit Types γ γ_db γ_s : gname.
 Implicit Types v : val.
-Implicit Types (ok : Prop) (failed : bool).
-Implicit Types si : sess_info.
+Implicit Types (failed : bool).
 
 Variable N : namespace.
 
-Definition dbCN kR := nroot.@"db".@"client".@kR.
-Definition dbSN kI := nroot.@"db".@"server".@kI.
-
-Definition failure kI kR : iProp :=
-  compromised_key kI ∨ compromised_key kR.
-
-Definition wf_sess_info si : iProp :=
-  minted (si_key si) ∗
-  senc_key (si_key si) ∗
-  key_secrecy si.
-
-#[global]
-Instance wf_sess_info_persistent cs : Persistent (wf_sess_info cs).
-Proof. apply _. Qed.
-
-Definition session_failed_for si rl (failed : bool) : iProp :=
-  term_meta (si_share_of rl si) (isoN.@"failed") failed ∗
-  (if failed then compromised_session si
-   else □ (public (si_key si) ↔ ▷ released_session si))%I.
-
-#[global]
-Instance session_failed_for_persistent si rl failed :
-  Persistent (session_failed_for si rl failed).
-Proof. by apply _. Qed.
-
-Lemma session_failed_for_agree si rl failed1 failed2 :
-  session_failed_for si rl failed1 -∗
-  session_failed_for si rl failed2 -∗
-  ⌜failed1 = failed2⌝.
-Proof.
-iIntros "(#meta1 & _) (#meta2 & _)".
-iApply (term_meta_agree with "meta1 meta2").
-Qed.
-
-Definition session_failed si failed : iProp :=
-  if failed then
-    (session_failed_for si Init true ∨
-     session_failed_for si Resp true)%I
-  else
-    (session_failed_for si Init false ∗
-     session_failed_for si Resp false)%I.
-
-Lemma session_failedI si failed1 failed2 :
-  session_failed_for si Init failed1 -∗
-  session_failed_for si Resp failed2 -∗
-  session_failed si (failed1 || failed2).
-Proof.
-iIntros "#? #?".
-case: failed1 => //=; eauto.
-case: failed2 => //=; eauto.
-Qed.
-
-Lemma session_failedI' si rl failed1 failed2 :
-  session_failed_for si rl failed1 -∗
-  session_failed_for si (swap_role rl) failed2 -∗
-  session_failed si (failed1 || failed2).
-Proof.
-iIntros "#failed1 #failed2". case: rl.
-- iApply (session_failedI with "failed1 failed2").
-- rewrite Bool.orb_comm. iApply (session_failedI with "failed2 failed1").
-Qed.
-
-Lemma session_okI si failed :
-  session_failed si failed -∗
-  (compromised_session si -∗ ▷ False) -∗
-  ◇ session_failed si false.
-Proof.
-case: failed => //; eauto.
-by iIntros "#[[_ fail1]|[_ fail2]] contra";
-iDestruct ("contra" with "[]") as ">[]".
-Qed.
-
-#[global]
-Instance session_failed_persistent si failed :
-  Persistent (session_failed si failed).
-Proof. apply _. Qed.
-
-Lemma session_failed_agree si failed1 failed2 :
-  session_failed si failed1 -∗
-  session_failed si failed2 -∗
-  ⌜failed1 = failed2⌝.
-Proof.
-iIntros "#failed1 #failed2".
-iAssert (session_failed si true -∗
-         session_failed si false -∗ False)%I
-  as "P".
-{ iIntros "#[fail|fail] #[succ1 succ2]".
-  - by iPoseProof (session_failed_for_agree with "fail succ1") as "%".
-  - by iPoseProof (session_failed_for_agree with "fail succ2") as "%". }
-case: failed1 failed2 => [] [] //.
-- by iDestruct ("P" with "failed1 failed2") as "[]".
-- by iDestruct ("P" with "failed2 failed1") as "[]".
-Qed.
-
-Lemma session_failed_forI cs (P : iProp) (failed : bool) :
-  wf_sess_info cs -∗
-  (if failed then compromised_session cs else P) -∗
-  term_token (cs_share cs) (↑isoN) ==∗ ∃ failed',
-  ⌜failed → failed'⌝ ∗
-  session_failed_for cs (cs_role cs) failed' ∗
-  (⌜failed'⌝ ∨ P) ∗
-  term_token (cs_share cs) (↑isoN ∖ ↑isoN.@"failed").
-Proof.
-iIntros "#wf HP token".
-iPoseProof "wf" as "(_ & _ & #? & [fail|#succ])".
-{ iMod (term_meta_set' true (N := isoN.@"failed") with "token")
-    as "[#failed token]" => //; try solve_ndisj.
-  iAssert (session_failed_for cs (cs_role cs) true) as "#?".
-  { iSplit => //. }
-  iExists true. iModIntro. iFrame. do !iSplit => //; eauto. }
-case: failed.
-{ iPoseProof "HP" as "#fail".
-  iMod (term_meta_set' true (N := isoN.@"failed") with "token")
-    as "[#failed token]" => //; try solve_ndisj.
-  iFrame "token". iModIntro. iExists true.
-  do !iSplit => //; eauto. }
-iMod (term_meta_set' false (N := isoN.@"failed") with "token")
-  as "[#failed token]" => //; try solve_ndisj.
-iAssert (session_failed_for cs (cs_role cs) false) as "#?".
-{ iSplit => //. iModIntro. by iSplit => //. }
-iFrame "token". iModIntro. iExists false.
-do !iSplit => //; eauto.
-Qed.
-
-Definition never_connected kI kR : iProp :=
-  term_token kR (↑dbSN kI).
-
-Lemma never_connected_switch kI kR Q : ⊢ switch (never_connected kI kR) Q.
-Proof. apply term_token_switch. Qed.
-
-Definition clock kI kR n :=
-  term_own kI (dbCN kR.@"status") (to_frac_agree (1 / 2) n).
-
-Lemma clock_alloc kI kR E :
-  ↑dbCN kR.@"status" ⊆ E →
-  term_token kI E ==∗
-  clock kI kR 0 ∗
-  clock kI kR 0 ∗
-  term_token kI (E ∖ ↑dbCN kR.@"status").
-Proof.
-iIntros "%sub token".
-iMod (term_own_alloc (dbCN kR.@"status") (to_frac_agree 1 0)
-       with "token") as "[own token]" => //.
-iFrame. rewrite -Qp.half_half frac_agree_op.
-iDestruct "own" as "[??]". by iFrame.
-Qed.
-
-Lemma clock_agree kI kR n m :
-  clock kI kR n -∗
-  clock kI kR m -∗
-  ⌜n = m⌝.
-Proof.
-iIntros "own1 own2".
-iPoseProof (term_own_valid_2 with "own1 own2") as "%valid".
-rewrite frac_agree_op_valid_L in valid.
-by case: valid.
-Qed.
-
-Lemma clock_update p kI kR n m :
-  clock kI kR n -∗
-  clock kI kR m ==∗
-  clock kI kR p ∗ clock kI kR p.
-Proof.
-iIntros "own1 own2".
-rewrite /clock.
-iMod (term_own_update_2 with "own1 own2") as "[own1 own2]".
-{ apply: (frac_agree_update_2 _ _ _ _ p).
-  by rewrite Qp.half_half. }
-by iFrame.
-Qed.
-
-Definition server_clock_ready kI kR :=
-  escrow (nroot.@"db") (never_connected kI kR)
-    (clock kI kR 0).
-
-Definition client_disconnected kI kR n failed : iProp :=
-  server_clock_ready kI kR ∗
-  if failed then failure kI kR else clock kI kR n.
-
 Definition db_disconnected kI kR : iProp := ∃ n failed,
-  DB.client_view kI (dbCN kR.@"state") n ∗
-  client_disconnected kI kR n failed.
-
-Definition client_disconnecting kI kR cs : iProp :=
-  ⌜cs_role cs = Init⌝ ∗
-  server_clock_ready kI kR ∗
-  term_token (si_init_share cs) (↑isoN.@"end").
-
-Definition connected kI kR cs n n0 : iProp :=
-  ⌜si_init cs = kI⌝ ∗
-  ⌜si_resp cs = kR⌝ ∗
-  wf_sess_info cs ∗
-  (∃ failed, session_failed_for cs (cs_role cs) failed) ∗
-  release_token (cs_share cs) ∗
-  cs_ts cs ↦ #n ∗
-  (∃ failed, session_failed cs failed) ∗
-  (session_failed cs true ∨
-     term_meta (si_init_share cs) (isoN.@"beginning") n0).
-
-Lemma connected_keyE kI kR cs n n0 :
-  connected kI kR cs n n0 -∗
-  ⌜kI = si_init cs⌝ ∗ ⌜kR = si_resp cs⌝.
-Proof. by iIntros "(-> & -> & _)". Qed.
-
-Definition client_token kI kR cs : iProp :=
-  ⌜cs_role cs = Init⌝ ∗
-  server_clock_ready kI kR ∗
-  term_token (si_init_share cs) (↑isoN.@"end").
+  DB.client_view kI (N.@"client".@kR.@"db") n ∗
+  Conn.client_disconnected N kI kR n failed.
 
 Definition db_connected kI kR cs : iProp := ∃ n n0,
-  DB.client_view kI (dbCN kR.@"state") (n + n0) ∗
-  connected kI kR cs n n0 ∗
-  client_token kI kR cs.
-
-Definition client_connecting cs n0 failed : iProp :=
-  let kI := si_init cs in
-  let kR := si_resp cs in
-  server_clock_ready kI kR ∗
-  wf_sess_info cs ∗
-  term_meta  (si_init_share cs) (isoN.@"beginning") n0 ∗
-  term_token (si_init_share cs) (↑isoN.@"end") ∗
-  session_failed_for cs Init failed.
-
-Lemma client_connecting_failed cs n0 failed :
-  client_connecting cs n0 failed -∗
-  session_failed_for cs Init failed.
-Proof. by iIntros "(_ & _ & _ & _ & ?)". Qed.
-
-Definition conn_ready si n :=
-  escrow (nroot.@"db")
-         (term_token (si_resp_share si) (↑isoN.@"begin"))
-         (clock (si_init si) (si_resp si) n).
-
-Lemma client_connectingI kI kR cs beginning failed :
-  si_init cs = kI →
-  si_resp cs = kR →
-  cs_role cs = Init →
-  cryptis_ctx -∗
-  £ 1 ∗ £ 1 -∗
-  wf_sess_info cs -∗
-  term_token (si_init_share cs) (↑isoN) -∗
-  client_disconnected kI kR beginning failed ={⊤}=∗ ∃ failed',
-  ⌜failed → failed'⌝ ∗
-  client_connecting cs beginning failed' ∗
-  term_meta (si_init_share cs) (isoN.@"beginning") beginning ∗
-  (⌜failed'⌝ ∨ conn_ready cs beginning).
-Proof.
-move=> <- <- e_rl {kI kR}.
-iIntros "#? [c1 c2] #sess token dis".
-iDestruct "dis" as "(#server & status)".
-have e_sh : si_init_share cs = cs_share cs by rewrite /cs_share e_rl.
-rewrite e_sh.
-iMod (session_failed_forI with "sess status token")
-  as "(%failed' & % & #conn & status & token)".
-iMod (term_meta_set' (N:=isoN.@"beginning") beginning with "token")
-  as "[#beginning token]"; try solve_ndisj.
-iExists failed'. iSplitR => //. iSplitL "token" => //.
-{ rewrite /client_connecting e_sh e_rl. iModIntro. do !iSplit => //.
-  rewrite (term_token_difference _ (↑isoN.@"end")); try solve_ndisj.
-  iDestruct "token" as "[token' token]". iFrame "token'". }
-iSplitR => //.
-iDestruct "status" as "[#?|status]"; eauto.
-iRight. iApply (escrowI with "status"). iApply term_token_switch.
-Qed.
-
-Lemma client_connectedI cs n0 failedI failedR :
-  cs_role cs = Init →
-  client_connecting cs n0 failedI -∗
-  cs_ts cs ↦ #0%nat -∗
-  release_token (si_init_share cs) -∗
-  session_failed_for cs Resp failedR ={⊤}=∗
-  ▷ (connected (si_init cs) (si_resp cs) cs 0 n0 ∗
-     client_token (si_init cs) (si_resp cs) cs).
-Proof.
-iIntros "%e_rl (#server & #? & ? & ? & #conn) ts rel #status".
-rewrite /connected /client_token /cs_share e_rl /=.
-iFrame. do 2!iModIntro. do 4!iSplit => //.
-iSplit; eauto.
-iExists (failedI || failedR).
-case: failedI => /=; eauto.
-case: failedR => /=; eauto.
-Qed.
-
-Lemma connected_ok kI kR cs n n0 :
-  connected kI kR cs n n0 -∗
-  (failure kI kR -∗ ▷ False) -∗
-  ◇ session_failed cs false.
-Proof.
-iIntros "(<- & <- & #conn & #? & rel & ts & #(%failed & status) & _) post".
-by iDestruct (session_okI with "status post") as ">?".
-Qed.
+  DB.client_view kI (N.@"client".@kR.@"db") (n + n0) ∗
+  Conn.connected kI kR cs n n0 ∗
+  Conn.client_token N kI kR cs.
 
 Lemma db_connected_ok kI kR cs :
   db_connected kI kR cs -∗
-  (failure kI kR -∗ ▷ False) -∗
-  ◇ session_failed cs false.
+  (Conn.failure kI kR -∗ ▷ False) -∗
+  ◇ Conn.session_failed cs false.
 Proof.
 iIntros "(% & % & ? & conn & _) fail".
-iApply (connected_ok with "conn fail").
+iApply (Conn.connected_ok with "conn fail").
 Qed.
 
 Definition rem_mapsto kI kR t1 t2 : iProp :=
-  DB.mapsto kI (dbCN kR.@"state") t1 t2.
+  DB.mapsto kI (N.@"client".@kR.@"db") t1 t2.
 
 Definition rem_free_at kI kR T : iProp :=
-  DB.free_at kI (dbCN kR.@"state") T.
+  DB.free_at kI (N.@"client".@kR.@"db") T.
 
 Lemma rem_free_at_diff kI kR T1 T2 :
   T1 ⊆ T2 →
@@ -398,11 +99,11 @@ Lemma rem_free_at_diff kI kR T1 T2 :
 Proof. iIntros "%sub". by iApply DB.free_at_diff. Qed.
 
 Lemma rem_mapsto_store t2' kI kR t1 t2 n :
-  DB.client_view kI (dbCN kR.@"state") n -∗
+  DB.client_view kI (N.@"client".@kR.@"db") n -∗
   rem_mapsto kI kR t1 t2 ==∗
-  DB.client_view kI (dbCN kR.@"state") (S n) ∗
+  DB.client_view kI (N.@"client".@kR.@"db") (S n) ∗
   rem_mapsto kI kR t1 t2' ∗
-  DB.store_at kI (dbCN kR.@"state") n t1 t2'.
+  DB.store_at kI (N.@"client".@kR.@"db") n t1 t2'.
 Proof.
 iIntros "client mapsto".
 iMod (DB.store_client t2' with "client mapsto")
@@ -412,12 +113,12 @@ Qed.
 
 Lemma rem_mapsto_alloc kI kR t1 t2 n T :
   t1 ∈ T →
-  DB.client_view kI (dbCN kR.@"state") n -∗
+  DB.client_view kI (N.@"client".@kR.@"db") n -∗
   rem_free_at kI kR T ==∗
-  DB.client_view kI (dbCN kR.@"state") (S n) ∗
+  DB.client_view kI (N.@"client".@kR.@"db") (S n) ∗
   rem_mapsto kI kR t1 t2 ∗
   rem_free_at kI kR (T ∖ {[t1]}) ∗
-  DB.create_at kI (dbCN kR.@"state") n t1 t2.
+  DB.create_at kI (N.@"client".@kR.@"db") n t1 t2.
 Proof.
 iIntros "%t1_T client".
 have {}t1_T : {[t1]} ⊆ T by set_solver.
@@ -428,29 +129,23 @@ iFrame. by eauto.
 Qed.
 
 Lemma client_alloc kI kR E :
-  ↑dbCN kR ⊆ E →
+  ↑N.@"client".@kR ⊆ E →
   term_token kI E ={⊤}=∗
   db_disconnected kI kR ∗
   rem_free_at kI kR ⊤ ∗
-  term_token kI (E ∖ ↑dbCN kR).
+  term_token kI (E ∖ ↑N.@"client".@kR).
 Proof.
 iIntros "%sub kI_token".
 rewrite (term_token_difference _ _ _ sub).
 iDestruct "kI_token" as "[kI_token ?]". iFrame.
-iMod (DB.alloc _ (N := dbCN kR.@"state") with "kI_token")
+iMod (Conn.client_alloc kI (kR := kR) with "kI_token")
+  as "[dis kI_token]" => //.
+{ solve_ndisj. }
+iMod (DB.alloc _ (N := N.@"client".@kR.@"db") with "kI_token")
   as "(client_view & free & #server_view & kI_token)".
 { solve_ndisj. }
-iMod (term_own_alloc (dbCN kR.@"status") (to_frac_agree 1 0)
-  with "kI_token") as "[status kI_token]" => //.
-{ solve_ndisj. }
-rewrite -Qp.half_half frac_agree_op.
-iDestruct "status" as "[client server]".
-iAssert (|={⊤}=> server_clock_ready kI kR)%I
-  with "[server]" as ">#server".
-{ iApply (escrowI with "server").
-  iApply never_connected_switch. }
 iModIntro. iSplitR "free".
-- iExists 0, false. by iFrame.
+- iExists 0, false. iFrame.
 - by iFrame.
 Qed.
 
@@ -471,30 +166,30 @@ case: (decide (t1' = t1)) => [-> {t1'} | ne].
 Qed.
 
 Definition server_token cs : iProp :=
-  session_failed cs true ∨ ∃ n0,
-    clock (si_init cs) (si_resp cs) n0 ∗
-    clock (si_init cs) (si_resp cs) n0.
+  Conn.session_failed cs true ∨ ∃ n0,
+    Conn.clock N (si_init cs) (si_resp cs) n0 ∗
+    Conn.clock N (si_init cs) (si_resp cs) n0.
 
 Definition server_db_connected' kI kR cs n n0 vdb : iProp :=
   ∃ db, public_db db ∗
         SAList.is_alist vdb (repr <$> db) ∗
-        (session_failed cs true ∨
-           DB.db_at kI (dbCN kR.@"state") (n + n0) db) ∗
+        (Conn.session_failed cs true ∨
+           DB.db_at kI (N.@"client".@kR.@"db") (n + n0) db) ∗
         server_token cs.
 
 Definition server_db_connected kI kR cs n n0 vdb : iProp :=
-  connected kI kR cs n n0 ∗
+  Conn.connected kI kR cs n n0 ∗
   server_db_connected' kI kR cs n n0 vdb.
 
 Definition server_disconnected kI kR n failed : iProp :=
-  if failed then failure kI kR
-  else (⌜n = 0⌝ ∗ never_connected kI kR ∨ clock kI kR n)%I.
+  if failed then Conn.failure kI kR
+  else (⌜n = 0⌝ ∗ Conn.never_connected N kI kR ∨ Conn.clock N kI kR n)%I.
 
 Definition server_db_disconnected' kI kR n vdb failed : iProp :=
   ∃ db,
     public_db db ∗
     SAList.is_alist vdb (repr <$> db) ∗
-    (⌜failed⌝ ∨ DB.db_at kI (dbCN kR.@"state") n db).
+    (⌜failed⌝ ∨ DB.db_at kI (N.@"client".@kR.@"db") n db).
 
 Definition server_db_disconnected kI kR vdb : iProp :=
   ∃ n failed,
@@ -502,198 +197,61 @@ Definition server_db_disconnected kI kR vdb : iProp :=
     server_db_disconnected' kI kR n vdb failed.
 
 Lemma server_db_alloc kI kR vdb E :
-  ↑dbSN kI ⊆ E →
+  ↑N.@"server".@kI ⊆ E →
   term_token kR E -∗
-  SAList.is_alist vdb ∅ -∗
-  term_token kR (E ∖ ↑dbSN kI) ∗
+  SAList.is_alist vdb ∅ ==∗
+  term_token kR (E ∖ ↑N.@"server".@kI) ∗
   server_db_disconnected kI kR vdb.
 Proof.
 iIntros "%sub token vdb".
-rewrite (term_token_difference kR (↑dbSN kI)) //.
-iDestruct "token" as "[token H]". iFrame "H".
-iExists 0, false. iSplitL "token".
-- iLeft. by iSplit => //.
-- iExists ∅. iFrame.
-  iSplit; first by rewrite /public_db big_sepM_empty.
-  iRight. iLeft. do !iSplit => //.
+iMod (Conn.server_alloc with "token") as "(dis & token)"; eauto.
+iModIntro. iFrame "token". iExists 0, false.
+iFrame. iExists ∅.
+iSplit; first by rewrite /public_db big_sepM_empty.
+iFrame. iRight. iLeft. do !iSplit => //.
 Qed.
 
 Definition server ss : iProp := ∃ accounts E,
   sign_key (ss_key ss) ∗
   SAList.is_alist (ss_clients ss) (repr <$> accounts) ∗
   term_token (ss_key ss) E ∗
-  ⌜∀ kI, TKey Open kI ∉ dom accounts → ↑dbSN kI ⊆ E⌝ ∗
+  ⌜∀ kI, TKey Open kI ∉ dom accounts → ↑N.@"server".@kI ⊆ E⌝ ∗
   [∗ map] vkI ↦ scs ∈ accounts, ∃ kI, ⌜vkI = TKey Open kI⌝ ∗
      is_lock (scs_name scs) (scs_lock scs)
        (server_db_disconnected kI (ss_key ss) (scs_db scs)).
 
 Lemma serverI kR vclients :
-  term_token kR (↑nroot.@"db".@"server") -∗
+  term_token kR (↑N.@"server") -∗
   sign_key kR -∗
   SAList.is_alist vclients ∅ -∗
   server {| ss_key := kR; ss_clients := vclients |}.
 Proof.
 iIntros "token #p_vk clients".
-iExists ∅, (↑nroot.@"db".@"server") => /=.
+iExists ∅, (↑N.@"server") => /=.
 iFrame. iSplit => //. iSplit => //.
 iPureIntro. move=> *. solve_ndisj.
 Qed.
 
-Definition session_msg_pred (Q : sess_info → term → iProp) rl kS m : iProp :=
-  ∃ si failed,
-    ⌜kS = (si_key si)⌝ ∗ public m ∗ session_failed_for si rl failed ∗
-    (⌜failed⌝ ∨ Q si m).
-
-Definition init_pred si t : iProp := ∃ (beginning : nat),
-  server_clock_ready (si_init si) (si_resp si) ∗
-  term_meta (si_init_share si) (isoN.@"beginning") beginning ∗
-  conn_ready si beginning.
-
-Lemma init_predI cs beginning failed m :
-  client_connecting cs beginning failed -∗
-  ⌜failed⌝ ∨ conn_ready cs beginning -∗
-  □ (⌜failed⌝ ∨ init_pred cs m).
-Proof.
-iIntros "(#server & #? & #? & ? & ? & #status) #[fail|ready]"; eauto.
-iModIntro. iRight. iExists _. eauto 10.
-Qed.
-
-Definition incoming_connection kR cs : iProp :=
-  wf_sess_info cs ∗
-  cs_ts cs ↦ #0%nat ∗
-  ⌜si_resp cs = kR⌝ ∗
-  ⌜cs_role cs = Resp⌝ ∗
-  release_token (cs_share cs) ∗
-  term_token (si_resp_share cs) (↑isoN) ∗
-  (∀ failed,
-     release_token (cs_share cs) -∗
-     session_failed_for cs (cs_role cs) failed ={⊤}=∗ ∃ failed',
-     ⌜failed → failed'⌝ ∗
-     release_token (cs_share cs) ∗
-     session_failed cs failed' ∗
-     (⌜failed'⌝ ∨ ∃ m, init_pred cs m)).
-
-Lemma server_connect kR cs n0 failed :
-  server_disconnected (si_init cs) kR n0 failed -∗
-  incoming_connection kR cs ={⊤}=∗
-  □ (⌜failed⌝ -∗ session_failed cs true) ∗
-  connected (si_init cs) kR cs 0 n0 ∗
-  server_token cs.
-Proof.
-iIntros "dis (#sess & ts & <- & %e_rl & rel & token & close)".
-have ->: si_resp_share cs = cs_share cs.
-{ by rewrite /cs_share e_rl. }
-iMod (session_failed_forI with "sess dis token")
-  as "(%failed' & %le_failed & #failed & dis & token)".
-iMod ("close" with "rel failed")
-  as "(%failed'' & %le_failed' & rel & #failed' & #init)".
-rewrite /connected /cs_share e_rl /=.
-rewrite (term_token_difference _ (↑isoN.@"begin")); try solve_ndisj.
-iDestruct "token" as "[token _]".
-iDestruct "dis" as "[%fail|dis]".
-{ iAssert (session_failed cs true) as "#?".
-  { by case: failed'' => //= in le_failed' *. }
-  iFrame. do !iSplitR => //; eauto. by iLeft. }
-iDestruct "init" as "[%fail|(%m & init)]".
-{ case: failed'' {le_failed'} => // in fail *.
-  iFrame. do !iSplitR => //; eauto. by iLeft. }
-iDestruct "init" as "(%n0' & clock & beginning & ready)".
-iMod (escrowE with "ready token") as ">c1" => //.
-iAssert (|={⊤}=> clock (si_init cs) (si_resp cs) n0)%I
-  with "[dis]" as "> c2".
-{ iDestruct "dis" as "[(-> & never)|c2]" => //.
-  iMod (escrowE with "clock never") as ">?" => //. }
-iPoseProof (clock_agree with "c1 c2") as "->".
-iModIntro. iFrame. do !iSplit => //; eauto.
-{ iIntros "!> %fail".
-  have: failed'' by tauto.
-  by case: (failed''). }
-iRight. iFrame.
-Qed.
-
-Definition ack_init_pred si t : iProp := True.
-
-Definition conn_pred φ kS m : iProp :=
-  ∃ si n ts,
-    ⌜kS = si_key si⌝ ∗
-    ⌜m = Spec.of_list (TInt n :: ts)⌝ ∗
-    ([∗ list] t ∈ ts, public t) ∗
-    (∃ failed, session_failed si failed) ∗
-    (session_failed si true ∨ ∃ n0,
-      term_meta (si_init_share si) (isoN.@"beginning") n0 ∗
-      φ (si_init si) (si_resp si) si (n + n0) ts).
-
-Lemma conn_predI kI kR cs m n0 φ n ts :
-  connected kI kR cs m n0 -∗
-  ([∗ list] t ∈ ts, public t) -∗
-  □ (session_failed cs true ∨ φ kI kR (cs_si cs) (n + n0) ts) -∗
-  □ conn_pred φ (si_key cs) (Spec.of_list (TInt n :: ts)).
-Proof.
-iIntros "(<- & <- & #conn & #? & _ & _ & #failed & #beginning)".
-iIntros "#p_ts #inv !>".
-iExists cs, n, ts.
-do 4!iSplit => //.
-iDestruct "beginning" as "[?|beginning]"; eauto.
-iDestruct "inv" as "[?|inv]"; eauto.
-Qed.
-
-Lemma conn_predE kI kR cs m n n0 φ ts :
-  connected kI kR cs m n0 -∗
-  □ conn_pred φ (si_key cs) (Spec.of_list (TInt n :: ts)) -∗
-  ([∗ list] t ∈ ts, public t) ∗
-  □ (session_failed cs true ∨ φ kI kR (cs_si cs) (n + n0) ts).
-Proof.
-iIntros "(<- & <- & #conn & #? & _ & _ & #failed & #beginning)".
-iIntros "#(%si & %n' & %ts' & %e_kS & %e_m & p_ts & failed' & inv)".
-case/Spec.of_list_inj: e_m => e_n <-.
-have {e_n} ?: n = n' by lia. subst n'.
-rewrite -(session_agree e_kS) {e_kS}.
-iSplit => //. iModIntro.
-iDestruct "beginning" as "[?|beginning]"; eauto.
-iDestruct "inv" as "[?|(%n0' & beginning' & inv)]"; eauto.
-iPoseProof (term_meta_agree with "beginning beginning'") as "<-".
-by iRight.
-Qed.
-
 Definition store_pred kI kR si n ts : iProp := ∃ t1 t2,
   ⌜ts = [t1; t2]⌝ ∗
-  DB.store_at kI (dbCN kR.@"state") n t1 t2.
+  DB.store_at kI (N.@"client".@kR.@"db") n t1 t2.
 
 Definition ack_store_pred kI kR si n ts : iProp := True.
 
 Definition load_pred kI kR si n ts : iProp :=
   ∃ t1, ⌜ts = [t1]⌝ ∗
-        DB.load_at kI (dbCN kR.@"state") n t1.
+        DB.load_at kI (N.@"client".@kR.@"db") n t1.
 
 Definition ack_load_pred kI kR si n ts : iProp :=
   ∃ t1 t2, ⌜ts = [t2]⌝ ∗
-    DB.load_at kI (dbCN kR.@"state") n t1 ∗
-    DB.stored_at kI (dbCN kR.@"state") (S n) t1 t2.
+    DB.load_at kI (N.@"client".@kR.@"db") n t1 ∗
+    DB.stored_at kI (N.@"client".@kR.@"db") (S n) t1 t2.
 
 Definition create_pred kI kR si n ts : iProp := ∃ t1 t2,
   ⌜ts = [t1; t2]⌝ ∗
-  DB.create_at kI (dbCN kR.@"state") n t1 t2.
+  DB.create_at kI (N.@"client".@kR.@"db") n t1 t2.
 
 Definition ack_create_pred kI kR si n ts : iProp := True.
-
-Definition close_pred kI kR si n ts : iProp :=
-  True.
-
-Definition conn_closed si ending :=
-  escrow (nroot.@"db")
-         (term_token (si_init_share si) (↑isoN.@"end"))
-         (clock (si_init si) (si_resp si) ending).
-
-Definition ack_close_pred kI kR si n ts : iProp :=
-  conn_closed si n.
-
-Lemma session_failed_failure si failed :
-  session_failed si failed ⊢ ⌜failed⌝ → compromised_session si.
-Proof.
-iIntros "#failed %fail".
-case: failed in fail * => //=.
-by iDestruct "failed" as "[[_ fail]|[_ fail]]".
-Qed.
 
 Definition server_handler_post kI kR cs n0 vdb v : iProp :=
   ⌜v = #true⌝ ∗
@@ -702,10 +260,12 @@ Definition server_handler_post kI kR cs n0 vdb v : iProp :=
 
 Lemma ack_load_predI skI skR cs n t1 t2 db :
   db !! t1 = Some t2 →
-  □ (session_failed cs true ∨ load_pred skI skR cs n [t1]) -∗
-  □ (session_failed cs true ∨ DB.db_at skI (dbCN skR.@"state") n db) -∗
-  (session_failed cs true ∨ □ ack_load_pred skI skR cs n [t2]) ∗
-  □ (session_failed cs true ∨ DB.db_at skI (dbCN skR.@"state") (S n) db).
+  □ (Conn.session_failed cs true ∨ load_pred skI skR cs n [t1]) -∗
+  □ (Conn.session_failed cs true ∨
+       DB.db_at skI (N.@"client".@skR.@"db") n db) -∗
+  (Conn.session_failed cs true ∨ □ ack_load_pred skI skR cs n [t2]) ∗
+  □ (Conn.session_failed cs true ∨
+       DB.db_at skI (N.@"client".@skR.@"db") (S n) db).
 Proof.
 iIntros "%db_t1 #[?|load] #[?|db_at]"; eauto.
 iDestruct "load" as "(%t1' & %e & load)".
@@ -718,17 +278,13 @@ iSplit; iRight.
 Qed.
 
 Definition store_ctx : iProp :=
-  seal_pred (N.@"init")       (session_msg_pred init_pred Init) ∗
-  seal_pred (N.@"ack_init")   (session_msg_pred ack_init_pred Resp) ∗
-  seal_pred (N.@"store")      (conn_pred store_pred) ∗
-  seal_pred (N.@"ack_store")  (conn_pred ack_store_pred) ∗
-  seal_pred (N.@"load")       (conn_pred load_pred) ∗
-  seal_pred (N.@"ack_load")   (conn_pred ack_load_pred) ∗
-  seal_pred (N.@"create")     (conn_pred create_pred) ∗
-  seal_pred (N.@"ack_create") (conn_pred ack_create_pred) ∗
-  seal_pred (N.@"close")      (conn_pred close_pred) ∗
-  seal_pred (N.@"ack_close")  (conn_pred ack_close_pred) ∗
-  iso_dh_ctx (N.@"auth").
+  seal_pred (N.@"store")      (Conn.conn_pred store_pred) ∗
+  seal_pred (N.@"ack_store")  (Conn.conn_pred ack_store_pred) ∗
+  seal_pred (N.@"load")       (Conn.conn_pred load_pred) ∗
+  seal_pred (N.@"ack_load")   (Conn.conn_pred ack_load_pred) ∗
+  seal_pred (N.@"create")     (Conn.conn_pred create_pred) ∗
+  seal_pred (N.@"ack_create") (Conn.conn_pred ack_create_pred) ∗
+  Conn.ctx N.
 
 Lemma store_ctx_alloc E :
   ↑N ⊆ E →
@@ -738,12 +294,6 @@ Proof.
 iIntros "%sub token".
 rewrite (seal_pred_token_difference (↑N)) => //.
 iDestruct "token" as "[token ?]". iFrame.
-iMod (seal_pred_set (N.@"init") with "token")
-  as "[init token]"; try solve_ndisj.
-iFrame.
-iMod (seal_pred_set (N.@"ack_init") with "token")
-  as "[ack_init token]"; try solve_ndisj.
-iFrame.
 iMod (seal_pred_set (N.@"store") with "token")
   as "[store token]"; try solve_ndisj.
 iFrame.
@@ -762,14 +312,8 @@ iFrame.
 iMod (seal_pred_set (N.@"ack_create") with "token")
   as "[ack_create token]"; try solve_ndisj.
 iFrame.
-iMod (seal_pred_set (N.@"close") with "token")
-  as "[close token]"; try solve_ndisj.
-iFrame.
-iMod (seal_pred_set (N.@"ack_close") with "token")
-  as "[ack_close token]"; try solve_ndisj.
-iFrame.
-iMod (iso_dh_ctx_alloc (N.@"auth") with "token")
-  as "#iso_dh"; try solve_ndisj.
+iMod (Conn.ctx_alloc (N := N) with "token")
+  as "(#iso_dh & ?)"; try solve_ndisj.
 Qed.
 
 Ltac solve_ctx :=
@@ -779,47 +323,31 @@ Ltac solve_ctx :=
     first [iApply "H" | iClear "H"]
   ).
 
-Lemma store_ctx_init :
-  store_ctx -∗ seal_pred (N.@"init") (session_msg_pred init_pred Init).
-Proof. solve_ctx. Qed.
-
-Lemma store_ctx_ack_init :
-  store_ctx -∗ seal_pred (N.@"ack_init") (session_msg_pred ack_init_pred Resp).
-Proof. solve_ctx. Qed.
-
 Lemma store_ctx_store :
-  store_ctx -∗ seal_pred (N.@"store") (conn_pred store_pred).
+  store_ctx -∗ seal_pred (N.@"store") (Conn.conn_pred store_pred).
 Proof. solve_ctx. Qed.
 
 Lemma store_ctx_ack_store :
-  store_ctx -∗ seal_pred (N.@"ack_store") (conn_pred ack_store_pred).
+  store_ctx -∗ seal_pred (N.@"ack_store") (Conn.conn_pred ack_store_pred).
 Proof. solve_ctx. Qed.
 
 Lemma store_ctx_load :
-  store_ctx -∗ seal_pred (N.@"load") (conn_pred load_pred).
+  store_ctx -∗ seal_pred (N.@"load") (Conn.conn_pred load_pred).
 Proof. solve_ctx. Qed.
 
 Lemma store_ctx_ack_load :
-  store_ctx -∗ seal_pred (N.@"ack_load") (conn_pred ack_load_pred).
+  store_ctx -∗ seal_pred (N.@"ack_load") (Conn.conn_pred ack_load_pred).
 Proof. solve_ctx. Qed.
 
 Lemma store_ctx_create :
-  store_ctx -∗ seal_pred (N.@"create") (conn_pred create_pred).
+  store_ctx -∗ seal_pred (N.@"create") (Conn.conn_pred create_pred).
 Proof. solve_ctx. Qed.
 
 Lemma store_ctx_ack_create :
-  store_ctx -∗ seal_pred (N.@"ack_create") (conn_pred ack_create_pred).
+  store_ctx -∗ seal_pred (N.@"ack_create") (Conn.conn_pred ack_create_pred).
 Proof. solve_ctx. Qed.
 
-Lemma store_ctx_close :
-  store_ctx -∗ seal_pred (N.@"close") (conn_pred close_pred).
-Proof. solve_ctx. Qed.
-
-Lemma store_ctx_ack_close :
-  store_ctx -∗ seal_pred (N.@"ack_close") (conn_pred ack_close_pred).
-Proof. solve_ctx. Qed.
-
-Lemma store_ctx_iso_dh_ctx : store_ctx -∗ iso_dh_ctx (N.@"auth").
+Lemma store_ctx_conn_ctx : store_ctx -∗ Conn.ctx N.
 Proof. solve_ctx. Qed.
 
 End Defs.
