conn.v
@@ -1,3 +1,4 @@
+From cryptis Require Import iso_dh.
 From cryptis.conn Require Import props impl proofs.
 
 Module Conn.
@@ -7,3 +8,5 @@ Include Impl.
 Include Proofs.
 
 End Conn.
+
+Coercion Conn.cs_si : Conn.state >-> sess_info.
