store/client_proofs/close.v
@@ -5,8 +5,8 @@ From iris.algebra Require Import agree auth csum gset gmap excl frac.
 From iris.algebra Require Import max_prefix_list.
 From iris.heap_lang Require Import notation proofmode.
 From cryptis Require Import lib version term gmeta nown cryptis.
-From cryptis Require Import primitives tactics role iso_dh.
-From cryptis.store Require Import impl shared db connection_proofs.
+From cryptis Require Import primitives tactics role iso_dh conn.
+From cryptis.store Require Import impl shared db.
 
 Set Implicit Arguments.
 Unset Strict Implicit.
@@ -19,7 +19,7 @@ Notation iProp := (iProp Σ).
 
 Context `{!storeG Σ}.
 
-Implicit Types (cs : conn_state).
+Implicit Types (cs : Conn.state).
 Implicit Types kI kR kS t : term.
 Implicit Types n : nat.
 Implicit Types γ : gname.
@@ -30,33 +30,33 @@ Variable N : namespace.
 Lemma wp_client_close c kI kR cs :
   channel c -∗
   store_ctx N -∗
-  {{{ db_connected kI kR cs }}}
+  {{{ db_connected N kI kR cs }}}
     Client.close N c (repr cs)
-  {{{ RET #(); db_disconnected kI kR }}}.
+  {{{ RET #(); db_disconnected N kI kR }}}.
 Proof.
 iIntros "#chan_c (_ & _ & _ & _ & _ & _ & _ & _ & #close & #ack & _)".
 iIntros "!> %Φ client post".
 iDestruct "client" as "(%n & %n0 & client & conn & token)".
-iPoseProof (connected_keyE with "conn") as "[-> ->]".
+iPoseProof (Conn.connected_keyE with "conn") as "[-> ->]".
 wp_lam. wp_pures.
 wp_apply (@wp_nil term).
-wp_apply (wp_connection_write with "[//] [] [] [] [$]") => //.
+wp_apply (Conn.wp_write with "[//] [] [] [] [$]") => //.
 - iRight. iModIntro. by eauto.
 iIntros "conn". wp_pures.
-wp_apply (wp_connection_read with "[//] [] [$]") => //.
+wp_apply (Conn.wp_read with "[//] [] [$]") => //.
 iIntros "%ts (conn & _ & #inv)".
 wp_pures.
 iAssert (|={⊤}=>
-  ∃ failed, client_disconnected (si_init cs) (si_resp cs) (n + n0) failed)%I
+  ∃ failed, Conn.client_disconnected N (si_init cs) (si_resp cs) (n + n0) failed)%I
   with "[token]" as ">(%failed & dis)".
 { iDestruct "token" as "(%e_rl & #server & end)".
   iDestruct "inv" as "[fail|inv]".
   - iExists true. iModIntro. iSplit => //.
-    by iApply (session_failed_failure with "fail").
+    by iApply (Conn.session_failed_failure with "fail").
   - iMod (escrowE with "inv end") as ">c1" => //.
     iExists false. iModIntro. iSplit => //. }
 iDestruct "conn" as "(_ & _ & _ & _ & rel & ts & _)".
-wp_apply (wp_connection_close with "[$]"). iIntros "_".
+wp_apply (Conn.wp_close with "[$]"). iIntros "_".
 iApply "post". by iFrame.
 Qed.
 
