store/client_proofs/connect.v
@@ -8,8 +8,8 @@ From iris.base_logic.lib Require Import invariants.
 From iris.heap_lang Require Import notation proofmode.
 From cryptis Require Import lib version term gmeta nown.
 From cryptis Require Import cryptis primitives tactics.
-From cryptis Require Import role iso_dh.
-From cryptis.store Require Import impl shared db connection_proofs.
+From cryptis Require Import role conn.
+From cryptis.store Require Import impl shared db.
 
 Set Implicit Arguments.
 Unset Strict Implicit.
@@ -22,7 +22,7 @@ Notation iProp := (iProp Σ).
 
 Context `{!storeG Σ}.
 
-Implicit Types (cs : conn_state).
+Implicit Types (cs : Conn.state).
 Implicit Types kI kR kS t : term.
 Implicit Types n : nat.
 Implicit Types γ : gname.
@@ -36,17 +36,18 @@ Lemma wp_client_connect c kI kR :
   store_ctx N -∗
   sign_key kI -∗
   public (TKey Open kR) -∗
-  {{{ db_disconnected kI kR }}}
+  {{{ db_disconnected N kI kR }}}
     Client.connect N c kI (TKey Open kR)
   {{{ cs, RET (repr cs);
-      db_connected kI kR cs }}}.
+      db_connected N kI kR cs }}}.
 Proof.
 iIntros "#chan_c #ctx #ctx'".
+iPoseProof (store_ctx_conn_ctx with "ctx'") as "?".
 iIntros "#p_ekI #p_ekR".
 iIntros "!> %Φ client post".
 iDestruct "client" as "(%n & %failed & db & dis)".
 wp_lam. wp_pures.
-iApply (wp_connection_connect with "[//] [//] [//] [//] [//] [$]") => //.
+iApply (Conn.wp_connect with "[//] [//] [//] [//] [//] [$]") => //.
 iIntros "!> %cs (conn & token)".
 iApply "post".
 by iFrame.
