store/client_proofs/load.v
@@ -7,8 +7,8 @@ From iris.base_logic Require Import invariants.
 From iris.heap_lang Require Import notation proofmode.
 From cryptis Require Import lib version term gmeta nown cryptis.
 From cryptis Require Import primitives tactics.
-From cryptis Require Import role iso_dh.
-From cryptis.store Require Import impl shared db connection_proofs.
+From cryptis Require Import role conn.
+From cryptis.store Require Import impl shared db.
 
 Set Implicit Arguments.
 Unset Strict Implicit.
@@ -32,27 +32,27 @@ Lemma wp_client_load c kI kR cs t1 t2 :
   channel c -∗
   store_ctx N -∗
   public t1 -∗
-  {{{ db_connected kI kR cs ∗
-      rem_mapsto kI kR t1 t2 }}}
+  {{{ db_connected N kI kR cs ∗
+      rem_mapsto N kI kR t1 t2 }}}
     Client.load N c (repr cs) t1
   {{{ t2', RET (repr t2');
-      db_connected kI kR cs ∗
-      rem_mapsto kI kR t1 t2 ∗
+      db_connected N kI kR cs ∗
+      rem_mapsto N kI kR t1 t2 ∗
       public t2' ∗
-      (session_failed cs true ∨ ⌜t2' = t2⌝) }}}.
+      (Conn.session_failed cs true ∨ ⌜t2' = t2⌝) }}}.
 Proof.
 iIntros "#chan_c #ctx #p_t1 !> %Φ [client mapsto] post".
 iDestruct "client" as "(%n & %n0 & db & conn & token)".
 wp_lam; wp_pures. wp_list.
 iMod (DB.load_client t1 with "db") as "[#load_at db]".
-iDestruct "ctx" as "(_ & _ & _ & _ & load & ack_load & _)".
-wp_apply (wp_connection_write with "chan_c load [] [] [$]").
+iDestruct "ctx" as "(_ & _ & load & ack_load & _)".
+wp_apply (Conn.wp_write with "chan_c load [] [] [$]").
 - by rewrite /=; eauto.
 - iRight. iIntros "!>". iExists _. by eauto.
 iIntros "conn". wp_pures.
-wp_apply (wp_connection_read with "chan_c [//] [$]").
+wp_apply (Conn.wp_read with "chan_c [//] [$]").
 iIntros "%ts (conn & #p_ts & #inv_ts)". wp_pures.
-wp_apply (wp_connection_tick with "conn"). iIntros "conn".
+wp_apply (Conn.wp_tick with "conn"). iIntros "conn".
 rewrite [repr_list ts]repr_listE.
 iDestruct "inv_ts" as "[fail|inv_ts]".
 - wp_pures. case: ts => [|t ts]; wp_pures.
