store/client_proofs/store.v
@@ -5,8 +5,8 @@ From iris.algebra Require Import agree auth csum gset gmap excl frac.
 From iris.algebra Require Import max_prefix_list.
 From iris.heap_lang Require Import notation proofmode.
 From cryptis Require Import lib version term cryptis primitives tactics.
-From cryptis Require Import role iso_dh.
-From cryptis.store Require Import impl shared db connection_proofs.
+From cryptis Require Import role conn.
+From cryptis.store Require Import impl shared db.
 
 Set Implicit Arguments.
 Unset Strict Implicit.
@@ -19,7 +19,7 @@ Notation iProp := (iProp Σ).
 
 Context `{!storeG Σ}.
 
-Implicit Types (cs : conn_state).
+Implicit Types (cs : Conn.state).
 Implicit Types kI kR kS t : term.
 Implicit Types n : nat.
 Implicit Types γ : gname.
@@ -32,23 +32,23 @@ Lemma wp_client_store c kI kR cs t1 t2 t2' :
   store_ctx N -∗
   public t1 -∗
   public t2' -∗
-  {{{ db_connected kI kR cs ∗ rem_mapsto kI kR t1 t2 }}}
+  {{{ db_connected N kI kR cs ∗ rem_mapsto N kI kR t1 t2 }}}
     Client.store N c (repr cs) t1 t2'
-  {{{ RET #(); db_connected kI kR cs ∗ rem_mapsto kI kR t1 t2' }}}.
+  {{{ RET #(); db_connected N kI kR cs ∗ rem_mapsto N kI kR t1 t2' }}}.
 Proof.
 iIntros "#chan_c #ctx #p_t1 #p_t2 !> %Φ [client mapsto] post".
 iDestruct "client" as "(%n & %n0 & db & conn & token)".
 wp_lam. wp_pures. wp_list.
-iMod (rem_mapsto_store t2' with "db mapsto") as "(db & mapsto & #store)".
-wp_apply (wp_connection_write with "[//] [] [] [] [$]").
+iMod (rem_mapsto_store N t2' with "db mapsto") as "(db & mapsto & #store)".
+wp_apply (Conn.wp_write with "[//] [] [] [] [$]").
 - by iApply store_ctx_store.
 - rewrite /=; eauto.
 - iRight. by iExists t1, t2'; eauto.
 iIntros "conn". wp_pures.
-wp_apply (wp_connection_read with "[//] [] [$]").
+wp_apply (Conn.wp_read with "[//] [] [$]").
 - by iApply store_ctx_ack_store.
 iIntros "%ts [conn _]". wp_pures.
-wp_apply (wp_connection_tick with "[$]"). iIntros "conn".
+wp_apply (Conn.wp_tick with "[$]"). iIntros "conn".
 iApply "post". by iFrame.
 Qed.
 
