store/server_proofs.v
@@ -6,8 +6,8 @@ From iris.algebra Require Import max_prefix_list.
 From iris.heap_lang Require Import notation proofmode.
 From iris.heap_lang.lib Require Import ticket_lock.
 From cryptis Require Import lib version term cryptis primitives tactics.
-From cryptis Require Import gmeta nown role iso_dh.
-From cryptis.store Require Import impl shared alist db connection_proofs.
+From cryptis Require Import gmeta nown role iso_dh conn.
+From cryptis.store Require Import impl shared alist db.
 From cryptis.store.server_proofs
   Require Import load store create close.
 
@@ -24,8 +24,8 @@ Notation iProp := (iProp Σ).
 
 Context `{!storeGS Σ}.
 
-Implicit Types (cs : conn_state).
-Implicit Types kI kR kS t : term.
+Implicit Types (cs : Conn.state).
+Implicit Types skI skR kS t : term.
 Implicit Types n : nat.
 Implicit Types γ : gname.
 Implicit Types v : val.
@@ -33,10 +33,10 @@ Implicit Types v : val.
 Variable N : namespace.
 
 Lemma wp_server_start c skR E :
-  ↑nroot.@"db".@"server" ⊆ E →
+  ↑N.@"server" ⊆ E →
   {{{ channel c ∗ sign_key skR ∗ term_token skR E }}}
     Server.start skR
-  {{{ ss, RET (repr ss); server ss }}}.
+  {{{ ss, RET (repr ss); server N ss }}}.
 Proof.
 iIntros "%sub %Ψ (#? & #? & token) post".
 wp_lam. wp_pures. wp_apply SAList.wp_empty => //.
@@ -49,23 +49,23 @@ iFrame.
 iModIntro.
 rewrite big_sepM_empty. iSplit => //.
 iPureIntro.
-move=> kI _. rewrite /dbSN. solve_ndisj.
+move=> kI _. solve_ndisj.
 Qed.
 
 Lemma wp_server_conn_handler_body c skI skR cs n n0 vdb :
-  cs_role cs = Resp →
+  Conn.cs_role cs = Resp →
   channel c -∗
   store_ctx N -∗
-  {{{ server_db_connected skI skR cs n n0 vdb }}}
+  {{{ server_db_connected N skI skR cs n n0 vdb }}}
     Server.conn_handler_body N c (repr cs) vdb
-  {{{ v, RET v; server_handler_post skI skR cs n0 vdb v }}}.
+  {{{ v, RET v; server_handler_post N skI skR cs n0 vdb v }}}.
 Proof.
 iIntros "% #chan_c #ctx !> %Φ (conn & db) post".
 wp_lam. wp_pures.
-rewrite !Connection.subst_select /=.
+rewrite !Conn.subst_select /=.
 iApply (wp_wand with "[conn db] post").
 iRevert "db".
-iApply wp_connection_select => //=; do !iSplitR => //.
+iApply Conn.wp_select => //=; do !iSplitR => //.
 - by iApply wp_server_handle_store.
 - by iApply wp_server_handle_load.
 - by iApply wp_server_handle_create.
@@ -73,11 +73,11 @@ iApply wp_connection_select => //=; do !iSplitR => //.
 Qed.
 
 Lemma wp_server_conn_handler c cs n n0 vdb vlock γlock :
-  cs_role cs = Resp →
+  Conn.cs_role cs = Resp →
   channel c -∗
-  is_lock γlock vlock (server_db_disconnected (si_init cs) (si_resp cs) vdb) -∗
+  is_lock γlock vlock (server_db_disconnected N (si_init cs) (si_resp cs) vdb) -∗
   store_ctx N -∗
-  {{{ server_db_connected (si_init cs) (si_resp cs) cs n n0 vdb ∗
+  {{{ server_db_connected N (si_init cs) (si_resp cs) cs n n0 vdb ∗
       locked γlock }}}
     Server.conn_handler N c (repr cs) vdb vlock
   {{{ RET #(); True }}}.
@@ -97,13 +97,13 @@ iIntros "!> %v [state|state]".
   by eauto.
 Qed.
 
-Lemma wp_server_find_client ss kI :
-  {{{ cryptis_ctx ∗ server ss }}}
-    Server.find_client (repr ss) (TKey Open kI)
+Lemma wp_server_find_client ss skI :
+  {{{ cryptis_ctx ∗ server N ss }}}
+    Server.find_client (repr ss) (TKey Open skI)
   {{{ vdb γlock vlock, RET (vdb, vlock)%V;
-      server ss ∗
+      server N ss ∗
       is_lock γlock vlock
-        (server_db_disconnected kI (ss_key ss) vdb) }}}.
+        (server_db_disconnected N skI (ss_key ss) vdb) }}}.
 Proof.
 iIntros "%Φ [#ctx server] post".
 iDestruct "server"
@@ -112,26 +112,26 @@ wp_lam; wp_pures.
 wp_bind (SAList.find _ _).
 iApply (SAList.wp_find with "accounts").
 iIntros "!> accounts"; rewrite lookup_fmap.
-case accounts_kI: (accounts !! TKey Open kI) => [scs|]; wp_pures.
+case accounts_skI: (accounts !! TKey Open skI) => [scs|]; wp_pures.
 - rewrite big_sepM_forall.
-  iPoseProof ("locks" $! (TKey Open kI) scs with "[//]")
-    as "(%kI' & %e & #lock)".
-  case: e => <- {kI'}.
+  iPoseProof ("locks" $! (TKey Open skI) scs with "[//]")
+    as "(%skI' & %e & #lock)".
+  case: e => <- {skI'}.
   iModIntro.
   iApply ("post" $! (scs_db scs) (scs_name scs) (scs_lock scs)).
   iSplit => //.
   iExists accounts, E. iFrame.
   rewrite big_sepM_forall. by eauto.
-- have ?: ↑dbSN kI ⊆ E.
-  { by apply: EP; rewrite elem_of_dom accounts_kI. }
-  rewrite (term_token_difference _ (↑dbSN kI)) //.
-  iDestruct "token" as "[token_kI token]".
+- have ?: ↑N.@"server".@skI ⊆ E.
+  { by apply: EP; rewrite elem_of_dom accounts_skI. }
+  rewrite (term_token_difference _ (↑N.@"server".@skI)) //.
+  iDestruct "token" as "[token_skI token]".
   wp_bind (SAList.new #()).
   iApply SAList.wp_empty => //.
   iIntros "!> %vdb db". wp_pures.
   wp_bind (newlock #()).
-  iDestruct (server_db_alloc with "token_kI db") as "[_ db]"; eauto.
-  iApply (newlock_spec (server_db_disconnected kI (ss_key ss) vdb)
+  iDestruct (server_db_alloc with "token_skI db") as ">[_ db]"; eauto.
+  iApply (newlock_spec (server_db_disconnected N skI (ss_key ss) vdb)
            with "[db]").
   { iFrame. }
   iIntros "!> %vlock %γlock #lock".
@@ -144,14 +144,14 @@ case accounts_kI: (accounts !! TKey Open kI) => [scs|]; wp_pures.
   iModIntro.
   iApply ("post" $! vdb γlock vlock).
   iSplit => //.
-  iExists _, (E ∖ ↑dbSN kI).
+  iExists _, (E ∖ ↑N.@"server".@skI).
   iFrame.
   do !iSplit => //.
   + iPureIntro.
-    move=> kI'.
+    move=> skI'.
     rewrite dom_insert elem_of_union elem_of_singleton.
     case/Decidable.not_or => fresh1 fresh2.
-    have ?: kI' ≠ kI by congruence.
+    have ?: skI' ≠ skI by congruence.
     move/(_ _ fresh2) in EP.
     solve_ndisj.
   + rewrite big_sepM_insert => //.
@@ -160,14 +160,14 @@ case accounts_kI: (accounts !! TKey Open kI) => [scs|]; wp_pures.
 Qed.
 
 Lemma wp_server_listen c ss :
-  {{{ cryptis_ctx ∗ channel c ∗ store_ctx N ∗ server ss }}}
+  {{{ cryptis_ctx ∗ channel c ∗ store_ctx N ∗ server N ss }}}
     Server.listen N c (repr ss)
-  {{{ RET #(); server ss }}}.
+  {{{ RET #(); server N ss }}}.
 Proof.
 iIntros "%Φ (#? & #chan_c & #ctx & server) post".
 wp_lam; wp_pures.
-iPoseProof (store_ctx_iso_dh_ctx with "ctx") as "dh".
-wp_apply (wp_connection_listen
+iPoseProof (store_ctx_conn_ctx with "ctx") as "?".
+wp_apply (Conn.wp_listen
          with "[# //] [# //] [# //] [#] []") => //;
   try by solve_ndisj.
 { by iDestruct "server" as "(% & % & ? & _)". }
@@ -182,12 +182,12 @@ iApply acquire_spec => //.
 iIntros "!> (locked & dis)".
 iDestruct "dis" as "(%n & %failed & dis & db_dis)".
 wp_pures.
-wp_apply (wp_connection_confirm with "[] [] [] [$]") => //.
+wp_apply (Conn.wp_confirm with "[] [] [] [$]") => //.
 iIntros "(%e_rl & #fail & conn & token)".
 wp_pures.
 iApply (wp_fork with "[db_dis conn token locked]").
 { iModIntro.
-  iDestruct (connected_keyE with "conn") as "#[_ ->]".
+  iDestruct (Conn.connected_keyE with "conn") as "#[_ ->]".
   wp_apply (wp_server_conn_handler
              with "[] [] [] [db_dis $conn $token $locked]") => //.
   iDestruct "db_dis" as "(%db & #p_db & db & #db_at)".
