store/server_proofs/close.v
@@ -5,8 +5,8 @@ From iris.algebra Require Import agree auth csum gset gmap excl frac.
 From iris.algebra Require Import max_prefix_list.
 From iris.heap_lang Require Import notation proofmode.
 From cryptis Require Import lib version term cryptis primitives tactics.
-From cryptis Require Import role iso_dh.
-From cryptis.store Require Import impl shared alist db connection_proofs.
+From cryptis Require Import role conn.
+From cryptis.store Require Import impl shared alist db.
 
 Set Implicit Arguments.
 Unset Strict Implicit.
@@ -19,7 +19,7 @@ Notation iProp := (iProp Σ).
 
 Context `{!storeGS Σ}.
 
-Implicit Types (cs : conn_state).
+Implicit Types (cs : Conn.state).
 Implicit Types kI kR kS t : term.
 Implicit Types n : nat.
 Implicit Types γ : gname.
@@ -30,49 +30,50 @@ Variable N : namespace.
 Ltac failure := iLeft; iFrame.
 
 Lemma wp_server_handle_close c skI skR cs n n0 vdb :
-  cs_role cs = Resp →
+  Conn.cs_role cs = Resp →
   channel c -∗
   store_ctx N -∗
-  handler_correct
-    (server_db_connected' skI skR cs n n0 vdb)
-    (server_handler_post skI skR cs n0 vdb)
+  Conn.handler_correct
+    (server_db_connected' N skI skR cs n n0 vdb)
+    (server_handler_post N skI skR cs n0 vdb)
     skI skR cs n n0
-    (N.@"close", Server.handle_close N c (repr cs) vdb).
+    (N.@"conn".@"close", Server.handle_close N c (repr cs) vdb).
 Proof.
 iIntros "%e_rl #chan_c #ctx".
-iPoseProof (store_ctx_close with "ctx") as "?".
-iPoseProof (store_ctx_ack_close with "ctx") as "?".
-rewrite /handler_correct /=. wp_lam; wp_pures. iModIntro.
+iPoseProof (store_ctx_conn_ctx with "ctx") as "{ctx} ctx".
+iPoseProof (Conn.ctx_close with "ctx") as "?".
+iPoseProof (Conn.ctx_ack_close with "ctx") as "?".
+rewrite /Conn.handler_correct /=. wp_lam; wp_pures. iModIntro.
 iExists _. iSplit => //.
 iIntros "!> %ts conn _ _ db". wp_pures.
 iDestruct "db" as "(%db & #p_db & vdb & #db_at & token)".
-iPoseProof (connected_keyE with "conn") as "%e".
+iPoseProof (Conn.connected_keyE with "conn") as "%e".
 iAssert (|={⊤}=>
-  (session_failed cs true ∨
-     □ ack_close_pred skI skR cs (n + n0) [TInt 0]) ∗
-  server_db_disconnected skI skR vdb)%I
+  (Conn.session_failed cs true ∨
+     □ Conn.ack_close_pred N skI skR cs (n + n0) [TInt 0]) ∗
+  server_db_disconnected N skI skR vdb)%I
   with "[vdb token]" as ">(#? & server)".
 { case: e => -> ->. iFrame.
   iDestruct "db_at" as "[fail|db_at]".
   { iModIntro. do !iSplit => //=; eauto.
     iExists (n + n0), true. do !iSplit => //=; eauto.
-    iApply (session_failed_failure cs true with "fail [//]"). }
+    iApply (Conn.session_failed_failure cs true with "fail [//]"). }
   iDestruct "token" as "[fail|(%n' & c1 & c2)]".
   { iModIntro. do !iSplit => //=; eauto.
     iExists (n + n0), true. do !iSplit => //=; eauto.
-    iApply (session_failed_failure cs true with "fail [//]"). }
-  iMod (clock_update (n + n0) with "c1 c2") as "[c1 c2]".
-  iAssert (|={⊤}=> conn_closed cs (n + n0))%I with "[c2]" as ">#?".
+    iApply (Conn.session_failed_failure cs true with "fail [//]"). }
+  iMod (Conn.clock_update N (n + n0) with "c1 c2") as "[c1 c2]".
+  iAssert (|={⊤}=> Conn.conn_closed N cs (n + n0))%I with "[c2]" as ">#?".
   { iApply (escrowI with "c2"). iApply term_token_switch. }
   iModIntro. iSplit; eauto.
   iExists (n + n0), false. do !iSplit => //; eauto.
   by iRight. }
 wp_list.
-wp_apply (wp_connection_write with "[//] [] [] [] [$]") => //.
+wp_apply (Conn.wp_write with "[//] [] [] [] [$]") => //.
 { by rewrite /= public_TInt; eauto. }
 iIntros "conn". wp_pures.
 iDestruct "conn" as "(? & ? & ? & ? & rel & ts & _)".
-wp_apply (wp_connection_close with "ts"). iIntros "_".
+wp_apply (Conn.wp_close with "ts"). iIntros "_".
 wp_pures. iModIntro. iRight. iExists _. iSplit => //.
 iRight. by iFrame.
 Qed.
