store/server_proofs/create.v
@@ -5,8 +5,8 @@ From iris.algebra Require Import agree auth csum gset gmap excl frac.
 From iris.algebra Require Import max_prefix_list.
 From iris.heap_lang Require Import notation proofmode.
 From cryptis Require Import lib version term cryptis primitives tactics.
-From cryptis Require Import role iso_dh.
-From cryptis.store Require Import impl shared alist db connection_proofs.
+From cryptis Require Import role conn.
+From cryptis.store Require Import impl shared alist db.
 
 Set Implicit Arguments.
 Unset Strict Implicit.
@@ -19,7 +19,7 @@ Notation iProp := (iProp Σ).
 
 Context `{!storeGS Σ}.
 
-Implicit Types (cs : conn_state).
+Implicit Types (cs : Conn.state).
 Implicit Types kI kR kS t : term.
 Implicit Types n : nat.
 Implicit Types γ : gname.
@@ -30,19 +30,19 @@ Variable N : namespace.
 Ltac failure := iLeft; iFrame; eauto.
 
 Lemma wp_server_handle_create c kI kR cs n n0 vdb :
-  cs_role cs = Resp →
+  Conn.cs_role cs = Resp →
   channel c -∗
   store_ctx N -∗
-  handler_correct
-    (server_db_connected' kI kR cs n n0 vdb)
-    (server_handler_post kI kR cs n0 vdb)
+  Conn.handler_correct
+    (server_db_connected' N kI kR cs n n0 vdb)
+    (server_handler_post N kI kR cs n0 vdb)
     kI kR cs n n0
     (N.@"create", Server.handle_create N c (repr cs) vdb).
 Proof.
 iIntros "%e_rl #chan_c #ctx".
 iPoseProof (store_ctx_create with "ctx") as "?".
 iPoseProof (store_ctx_ack_create with "ctx") as "?".
-rewrite /handler_correct /=. wp_lam; wp_pures.
+rewrite /Conn.handler_correct /=. wp_lam; wp_pures.
 iModIntro. iExists _. iSplit => //.
 iIntros "!> %ts conn #p_ts #inv_ts db".
 iDestruct "db" as "(%db & #p_db & db & #db_at & token)".
@@ -52,8 +52,8 @@ wp_bind (SAList.find _ _). iApply (SAList.wp_find with "db") => //.
 iIntros "!> db". rewrite lookup_fmap.
 wp_bind (match: _ with InjL <> => _ | InjR <> => _ end)%E.
 iApply (wp_frame_wand with "conn").
-iAssert (session_failed cs true ∨
-           DB.db_at kI (dbCN kR.@"state")
+iAssert (Conn.session_failed cs true ∨
+           DB.db_at kI (N.@"client".@kR.@"db")
              (S n + n0) (DB.op_app db (Create t1 t2)))%I
   as "#db_at'".
 { iDestruct "inv_ts" as "[?|inv_ts]"; eauto.
@@ -63,7 +63,7 @@ iAssert (session_failed cs true ∨
   iRight. by iApply (DB.db_at_create_at with "db_at"). }
 iApply (wp_wand _ _ _ (λ v,
   ∃ (b : bool), ⌜v = #((if b then 1 else 0) : Z)⌝ ∗
-                server_db_connected' kI kR cs (S n) n0 vdb
+                server_db_connected' N kI kR cs (S n) n0 vdb
   ) with "[db token]")%I.
 { case db_t1: (db !! t1) => [t2'|]; wp_pures.
   { iExists false; iModIntro; iFrame.
@@ -81,12 +81,12 @@ wp_pures.
 wp_bind (tint _). iApply wp_tint.
 wp_list.
 wp_pures.
-wp_apply (wp_connection_write with "[//] [] [] [] [$]") => //.
+wp_apply (Conn.wp_write with "[//] [] [] [] [$]") => //.
 - rewrite /= public_TInt. iDestruct "p_ts" as "(? & ? & _)".
   by eauto.
 - by iRight.
 iIntros "conn". wp_pures.
-wp_apply (wp_connection_tick with "[$]"). iIntros "conn".
+wp_apply (Conn.wp_tick with "[$]"). iIntros "conn".
 wp_pures.
 iModIntro. iRight. iExists _. iSplit => //.
 iLeft. iSplit => //. iExists (S n). by iFrame.
