store/server_proofs/load.v
@@ -6,8 +6,8 @@ From iris.algebra Require Import max_prefix_list.
 From iris.heap_lang Require Import notation proofmode.
 From cryptis Require Import lib version term gmeta nown.
 From cryptis Require Import cryptis primitives tactics.
-From cryptis Require Import role iso_dh.
-From cryptis.store Require Import impl shared alist db connection_proofs.
+From cryptis Require Import role conn.
+From cryptis.store Require Import impl shared alist db.
 
 Set Implicit Arguments.
 Unset Strict Implicit.
@@ -20,8 +20,8 @@ Notation iProp := (iProp Σ).
 
 Context `{!storeGS Σ}.
 
-Implicit Types (cs : conn_state).
-Implicit Types kI kR kS t : term.
+Implicit Types (cs : Conn.state).
+Implicit Types skI skR kS t : term.
 Implicit Types n : nat.
 Implicit Types γ : gname.
 Implicit Types v : val.
@@ -31,19 +31,19 @@ Variable N : namespace.
 Ltac failure := iLeft; iFrame; eauto.
 
 Lemma wp_server_handle_load c skI skR cs n n0 vdb :
-  cs_role cs = Resp →
+  Conn.cs_role cs = Resp →
   channel c -∗
   store_ctx N -∗
-  handler_correct
-    (server_db_connected' skI skR cs n n0 vdb)
-    (server_handler_post skI skR cs n0 vdb)
+  Conn.handler_correct
+    (server_db_connected' N skI skR cs n n0 vdb)
+    (server_handler_post N skI skR cs n0 vdb)
     skI skR cs n n0
     (N.@"load", Server.handle_load N c (repr cs) vdb).
 Proof.
 iIntros "%e_rl #chan_c #ctx".
 iPoseProof (store_ctx_load with "ctx") as "?".
 iPoseProof (store_ctx_ack_load with "ctx") as "?".
-rewrite /handler_correct /=. wp_lam; wp_pures.
+rewrite /Conn.handler_correct /=. wp_lam; wp_pures.
 iModIntro. iExists _. iSplit => //.
 iIntros "!> %ts conn #p_ts #inv_ts (%db & #p_db & db & #db_at & token)".
 wp_pures.
@@ -53,12 +53,12 @@ iIntros "!> db". rewrite lookup_fmap.
 case db_t1: (db !! t1) => [t2|]; wp_pures; last by failure.
 wp_list.
 iPoseProof (ack_load_predI with "inv_ts db_at") as "[? #?]" => //.
-wp_apply (wp_connection_write with "[//] [] [] [] [$]") => //.
+wp_apply (Conn.wp_write with "[//] [] [] [] [$]") => //.
 - rewrite /public_db big_sepM_forall.
   iDestruct ("p_db" $! t1 t2 with "[//]") as "[??]".
   by rewrite /=; eauto.
 iIntros "conn". wp_pures.
-wp_apply (wp_connection_tick with "conn"). iIntros "conn". wp_pures.
+wp_apply (Conn.wp_tick with "conn"). iIntros "conn". wp_pures.
 iModIntro. iRight. iExists _. iSplit => //.
 iLeft. iSplit => //. iExists (S n). iFrame.
 by iSplit => //.
