store/server_proofs/store.v
@@ -5,8 +5,8 @@ From iris.algebra Require Import agree auth csum gset gmap excl frac.
 From iris.algebra Require Import max_prefix_list.
 From iris.heap_lang Require Import notation proofmode.
 From cryptis Require Import lib version term cryptis primitives tactics.
-From cryptis Require Import role iso_dh.
-From cryptis.store Require Import impl shared alist db connection_proofs.
+From cryptis Require Import role conn.
+From cryptis.store Require Import impl shared alist db.
 
 Set Implicit Arguments.
 Unset Strict Implicit.
@@ -19,7 +19,7 @@ Notation iProp := (iProp Σ).
 
 Context `{!storeGS Σ}.
 
-Implicit Types (cs : conn_state).
+Implicit Types (cs : Conn.state).
 Implicit Types kI kR kS t : term.
 Implicit Types n : nat.
 Implicit Types γ : gname.
@@ -30,19 +30,19 @@ Variable N : namespace.
 Ltac failure := iLeft; iFrame.
 
 Lemma wp_server_handle_store c kI kR cs n n0 vdb :
-  cs_role cs = Resp →
+  Conn.cs_role cs = Resp →
   channel c -∗
   store_ctx N -∗
-  handler_correct
-    (server_db_connected' kI kR cs n n0 vdb)
-    (server_handler_post kI kR cs n0 vdb)
+  Conn.handler_correct
+    (server_db_connected' N kI kR cs n n0 vdb)
+    (server_handler_post N kI kR cs n0 vdb)
     kI kR cs n n0
     (N.@"store", Server.handle_store N c (repr cs) vdb).
 Proof.
 iIntros "%e_rl #chan_c #ctx".
 iPoseProof (store_ctx_store with "ctx") as "?".
 iPoseProof (store_ctx_ack_store with "ctx") as "?".
-rewrite /handler_correct /=. wp_lam; wp_pures.
+rewrite /Conn.handler_correct /=. wp_lam; wp_pures.
 iModIntro. iExists _. iSplit => //.
 iIntros "!> %ts conn #p_ts #inv_m db". wp_pures.
 wp_list_match => [t1 t2 ->|_]; wp_pures; last by failure.
@@ -52,10 +52,10 @@ iApply (SAList.wp_insert with "db").
 iIntros "!> db". rewrite -fmap_insert.
 wp_pures.
 wp_apply (@wp_nil term).
-wp_apply (wp_connection_write with "[] [] [] [] [$]") => //.
+wp_apply (Conn.wp_write with "[] [] [] [] [$]") => //.
 { iRight. by eauto. }
 iIntros "conn". wp_pures. 
-wp_apply (wp_connection_tick with "[$]"). iIntros "conn". wp_pures.
+wp_apply (Conn.wp_tick with "[$]"). iIntros "conn". wp_pures.
 iModIntro. iRight. iExists _. iSplit => //.
 iLeft. iSplit => //. iExists (S n). iFrame.
 rewrite /=.
